verif/btrees/verif_findindex.v
@@ -22,13 +22,13 @@ unfold Int64.ltu in H. if_tac in H; inv H; auto.
 Qed.
 
 
-Lemma FCI_increase: forall X (le:listentry X) key i,
+Lemma FCI_increase: forall X (le:list (entry X)) key i,
     i <= findChildIndex' le key i.
 Proof.
   intros. generalize dependent i.
   induction le; intros.
   - simpl. omega.
-  - destruct e; simpl.
+  - destruct a; simpl.
     * destruct (k_ key <? k_ k). omega.
       eapply Z.le_trans with (m:= Z.succ i). omega.
       apply IHle.
@@ -37,7 +37,7 @@ Proof.
       apply IHle.
 Qed.
 
-Lemma FCI'_next_index {X: Type} (le: listentry X) key i:
+Lemma FCI'_next_index {X: Type} (le: list (entry X)) key i:
   findChildIndex' le key (Z.succ i) = Z.succ (findChildIndex' le key i).
 Proof.
   revert i.
@@ -45,7 +45,7 @@ Proof.
     destruct (k_ key <? k_ k); easy.
 Qed.  
 
-Lemma FRI'_next_index {X: Type} (le: listentry X) key i:
+Lemma FRI'_next_index {X: Type} (le: list (entry X)) key i:
   findRecordIndex' le key (Z.succ i) = Z.succ (findRecordIndex' le key i).
 Proof.
   revert i.
@@ -59,28 +59,29 @@ Proof.
   intros X n key.
   destruct n as [ptr0 le isLeaf F L x]; simpl.
   induction le. easy. simpl.
-  destruct e as [k v x'|k n]; destruct (k_ key <? k_ k);
+  autorewrite with sublist.
+  destruct a as [k v x'|k n]; destruct (k_ key <? k_ k);
   replace (findChildIndex' le key 0) with (Z.succ (findChildIndex' le key (-1))) by now rewrite <- FCI'_next_index.
   all: destruct (findChildIndex' le key (-1)); unfold  findChildIndex' in IHle |- *; omega.
 Qed.
 
-Lemma FCI_inrange'': forall X (le:listentry X) key j i,
+Lemma FCI_inrange'': forall X (le:list (entry X)) key j i,
     findChildIndex' le key j = i ->
     j <= i.
 Proof.
   intros.
   revert j H; induction le; simpl; intros. omega.
-  destruct e as [k v x'|k n]; destruct (k_ key <? k_ k); simpl in *; try omega.
+  destruct a as [k v x'|k n]; destruct (k_ key <? k_ k); simpl in *; try omega.
   1,2: apply IHle in H; omega.
 Qed.
 
-Lemma FRI_increase: forall X (le:listentry X) key i,
+Lemma FRI_increase: forall X (le:list (entry X)) key i,
     i <= findRecordIndex' le key i.
 Proof.
   intros. generalize dependent i.
   induction le; intros.
   - simpl. omega.
-  - destruct e; simpl.
+  - destruct a; simpl.
     * destruct (k_ key <=? k_ k). omega.
       eapply Z.le_trans with (m:= Z.succ i). omega.
       apply IHle.
@@ -94,12 +95,12 @@ Lemma FRI_inrange: forall X (n:node X) key,
 Proof.
   intros X n key.
    destruct n as [ptr0 le isLeaf F L x]; simpl.
-  rewrite <- (Z.add_0_r (numKeys_le le)).
+  rewrite <- (Z.add_0_r (Zlength le)).
   forget 0 as i.
   revert i; induction le; intros. easy.
-  simpl.
-  pose proof (numKeys_le_nonneg le).
-  destruct (k_ key <=? k_ (entry_key e)); try easy; try omega.
+  simpl. autorewrite with sublist.
+  pose proof (Zlength_nonneg le).
+  destruct (k_ key <=? k_ (entry_key a)); try easy; try omega.
   specialize (IHle (Z.succ i));   omega.
 Qed.
 
@@ -120,7 +121,7 @@ Proof.
   - elimtype False.
      destruct (intern_le_cons _ _ _ _ _ _ H0 I) as [le' [l2'' ?]].
      subst. simpl in H. apply node_wf_numKeys in H1. simpl in H1. 
-     normalize in H. pose proof (numKeys_le_nonneg l2''). rep_omega.
+     normalize in H. autorewrite with sublist in H. rep_omega.
   - destruct le as [|e le'] eqn:HLE.
     { apply intern_le_cons in H0. destruct H0. destruct H. inv H. simpl. auto. }
     destruct e eqn:HE.
@@ -130,12 +131,12 @@ Proof.
     forward.                    (* t'6=node->entries[0]->key *)
     change (?A :: ?B ++ ?C) with ((A::B)++C).
     change ((key_repr k, inl (getval n0)) :: _) with
-        (map entry_val_rep (le_to_list (cons val (keychild val k n0) le'))).
+        (map entry_val_rep (keychild val k n0 :: le')).
    change (btnode_rep n0) with (entry_rep (keychild val k n0)).
     sep_apply cons_le_iter_sepcon.
     change Vfalse with (Val.of_bool false).
     sep_apply (fold_btnode_rep ptr0). fold n.
-    deadvars!.      
+    deadvars!.
 {  forward_loop (EX i:Z, PROP(0 <= i <= numKeys n; findChildIndex' le key (-1) = findChildIndex' (skipn_le le i) key (Z.pred i)) 
                                      LOCAL(temp _i (Vint(Int.repr i)); temp _node pn; temp _key (key_repr key))
                                      SEP(btnode_rep n))
@@ -143,15 +144,15 @@ Proof.
                                         LOCAL(temp _i (Vint(Int.repr i)); temp _node pn; temp _key (key_repr key))
                                         SEP(btnode_rep n)).
 
-  - Exists 0.
-    entailer!. split. omega. apply numKeys_le_nonneg.
+  - Exists 0. unfold skipn_le; autorewrite with sublist.
+    entailer!. split. omega. apply Zlength_nonneg.
   - Intros i. clear ent_end ent_end0.
     rewrite unfold_btnode_rep. unfold n. Intros ent_end.
     forward.                    (* t'5=node->numKeys *)
-    sep_apply (fold_btnode_rep ptr0 (cons val (keychild val k n0) le')  false). fold n.
+    sep_apply (fold_btnode_rep ptr0 (keychild val k n0 :: le')  false). fold n.
     forward_if.
     + clear ent_end. rewrite unfold_btnode_rep. unfold n. Intros ent_end.
-      assert(HRANGE: 0 <= i < numKeys_le le).
+      assert(HRANGE: 0 <= i < Zlength le).
       { apply node_wf_numKeys in H1. simpl in H1.
         unfold n in H; simpl in H. rewrite HLE. simpl.
         rewrite !Int.signed_repr in H3 by rep_omega. omega. }
@@ -160,20 +161,21 @@ Proof.
       destruct NTHENTRY as [ei NTHENTRY].
       assert(ZNTH: nth_entry_le i le = Some ei) by auto.
       apply Znth_to_list' with (endle:=ent_end) in ZNTH. 
-      assert (H99: 0 <= numKeys_le le <= Fanout). {
+      assert (H99: 0 <= Zlength le <= Fanout). {
          clear - HLE H1. subst le. apply (node_wf_numKeys _ H1).
      }
       forward.                  (* t'2=node->entries+i->key *)
       { apply prop_right. rep_omega. }
-      { entailer!. simpl in ZNTH. rewrite ZNTH. destruct ei; simpl; auto. }
-      rewrite HLE in ZNTH. rewrite ZNTH.
+      { entailer!. simpl in ZNTH. fold Inhabitant_entry_val_rep.
+        rewrite ZNTH. destruct ei; simpl; auto. }
+      rewrite HLE in ZNTH.  fold Inhabitant_entry_val_rep. rewrite ZNTH.
       forward_if.
       * forward.                (* return i-1 *)
         entailer!.
         { simpl cast_int_int.  normalize. f_equal. f_equal.
-          change (i-1 = findChildIndex' (cons val (keychild val k n0) le') key (-1)).
+          change (i-1 = findChildIndex' (keychild val k n0 :: le') key (-1)).
           rewrite H2.
-          set (le:=cons val (keychild val k n0) le') in NTHENTRY|-*.
+          set (le:=keychild val k n0 :: le') in NTHENTRY|-*.
           clear -NTHENTRY H4 HRANGE.
           assert(k_ key <? k_ (entry_key ei) = true).
           { assert(-1 < k_ key < Ptrofs.modulus) by (unfold k_; rep_omega).
@@ -185,14 +187,15 @@ Proof.
             apply H4. } clear H4.
           apply nth_entry_skipn in NTHENTRY.
           destruct (skipn_le le i); inv NTHENTRY. 
+           autorewrite with sublist in H1. inv H1.
           destruct ei; simpl in H; simpl; rewrite H; normalize; f_equal. }
-          rewrite unfold_btnode_rep with (n:= btnode val ptr0 (cons val (keychild val k n0) le') false First Last pn).
+          rewrite unfold_btnode_rep with (n:= btnode val ptr0 (keychild val k n0 :: le') false First Last pn).
         Exists ent_end. cancel.
       * forward.                (* i++ *)
         Exists (Z.succ i). entailer!. split.
         { clear - HRANGE H1. subst n. simpl in *. omega. }
         { rewrite H2.
-          pose (le:=cons val (keychild val k n0) le').
+          pose (le:= keychild val k n0 :: le').
           fold le. fold le in NTHENTRY. clear -NTHENTRY H4 HRANGE.
           assert(k_ key <? k_ (entry_key ei) = false).
           { assert(-1 < k_ key < Int64.modulus) by (unfold k_; rep_omega).
@@ -202,10 +205,11 @@ Proof.
               rewrite ?int_unsigned_ptrofs_toint in H4 by reflexivity;
               rewrite ?int64_unsigned_ptrofs_toint in H4 by reflexivity;
               omega. }
-          apply nth_entry_skipn in NTHENTRY.          
-          rewrite skip_S.
-          destruct (skipn_le le i); simpl in NTHENTRY; inv NTHENTRY.
-          assert(findChildIndex' (cons val ei l) key (Z.pred i) = findChildIndex' l key (Z.succ (Z.pred i))).
+          autorewrite with sublist in HRANGE.
+          apply nth_entry_skipn in NTHENTRY.
+          rewrite skip_S. 
+          destruct (skipn_le le i); autorewrite with sublist in NTHENTRY; inv NTHENTRY.
+          assert(findChildIndex' (ei :: l) key (Z.pred i) = findChildIndex' l key (Z.succ (Z.pred i))).
           { simpl; destruct ei; simpl in H; rewrite H; simpl; auto. } rewrite H0.
           simpl. f_equal. omega. omega. }
         do 2 f_equal. replace 1 with (Z.of_nat 1) by reflexivity.
@@ -215,18 +219,21 @@ Proof.
       unfold n in H. unfold node_wf in H1. simpl in H, H1.
       rewrite Int.signed_repr in H3 by rep_omega.
       rewrite Int.signed_repr in H3 by rep_omega.
-      assert( i = Z.succ (numKeys_le le')) by omega.
+      autorewrite with sublist in H3,H.
+      assert( i = Z.succ (Zlength le')) by omega.
       Exists i. entailer!.
-      rewrite H2. simpl.
-      rewrite zle_false by (pose proof (numKeys_le_nonneg le'); omega).
+      split. simpl. autorewrite with sublist. auto.
+      rewrite H2.     
       rewrite Z.pred_succ.
-      rewrite skipn_full. simpl. auto. 
+      replace (Z.succ (Zlength le')) with (Zlength (keychild val k n0 :: le')).
+      rewrite skipn_full. simpl. auto.
+      list_solve.
   - Intros i. clear ent_end ent_end0.
     rewrite unfold_btnode_rep. unfold n. Intros ent_end.
     forward.                     (* t'1=node->numKeys *)
     forward.                     (* return t'1-1 *)
     + entailer!. unfold node_wf in H1. simpl in H1.
-      pose proof (numKeys_le_nonneg le').
+      pose proof (Zlength_nonneg le').
       rewrite Int.signed_repr by rep_omega.
       rewrite Int.signed_repr by rep_omega.
       rep_omega.
@@ -234,7 +241,7 @@ Proof.
       * simpl cast_int_int; normalize.
         do 2 f_equal.
         unfold findChildIndex. rewrite H2. simpl numKeys. omega.
-      * rewrite unfold_btnode_rep with (n:=btnode val ptr0 (cons val (keychild val k n0) le') false First Last pn).
+      * rewrite unfold_btnode_rep with (n:=btnode val ptr0 (keychild val k n0 :: le') false First Last pn).
         Exists ent_end. cancel.  }
 Qed.
 
@@ -261,7 +268,7 @@ Proof.
     apply node_wf_numKeys in H0. simpl in H0.
     apply (f_equal Int.unsigned) in H1.  normalize in H1.
     f_equal. destruct le. simpl; auto. simpl in H1.
-    pose proof (numKeys_le_nonneg le); omega.
+    autorewrite with sublist in H1; rep_omega.
     rewrite unfold_btnode_rep with (n:=btnode val ptr0 le isLeaf First Last pn).
     Exists ent_end. entailer!. }
   forward.                    (* i=0 *)
@@ -275,7 +282,7 @@ Proof.
                                     LOCAL (temp _i (Vint (Int.repr i)); temp _node pn; temp _key (key_repr key))
                                     SEP (btnode_rep n)).
   - Exists 0. entailer!.
-    split. split. omega. apply numKeys_le_nonneg.
+    split. split. omega. apply Zlength_nonneg.
     rewrite skipn_0. auto.
   - Intros i. rewrite unfold_btnode_rep. unfold n. Intros ent_end.
     forward.                    (* t'3=node->numKeys *)
@@ -286,7 +293,7 @@ Proof.
       rewrite Int.signed_repr by rep_omega.
       rep_omega.
     + apply node_wf_numKeys in H0; simpl in H0. unfold n in H2; simpl in H2.
-        assert(HRANGE: 0 <= i < numKeys_le le).
+        assert(HRANGE: 0 <= i < Zlength le).
       { rewrite !Int.signed_repr in H4 by rep_omega. omega. }
       assert(NTHENTRY: exists ei, nth_entry_le i le = Some ei).
       { apply nth_entry_le_in_range. auto. }
@@ -295,8 +302,9 @@ Proof.
       apply Znth_to_list' with (endle:=ent_end) in ZNTH.
       forward.                  (* t'2=node->entries[i]->key *)
       { entailer!. }
-      { entailer!. rewrite ZNTH. destruct ei; simpl; auto. }
-      rewrite ZNTH.
+      { entailer!. 
+        fold Inhabitant_entry_val_rep. rewrite ZNTH. destruct ei; simpl; auto. }
+      fold Inhabitant_entry_val_rep. rewrite ZNTH.
       forward_if.
       * forward.                (* return i *)
         entailer!. unfold findRecordIndex. rewrite H3.
@@ -304,7 +312,9 @@ Proof.
         destruct (skipn_le le i) eqn:HSKIP.
         { simpl. auto. }
         apply nth_entry_skipn in NTHENTRY.
-        simpl in  NTHENTRY. rewrite HSKIP in NTHENTRY. inv NTHENTRY.
+        simpl in  NTHENTRY. rewrite HSKIP in NTHENTRY.
+        autorewrite with sublist in NTHENTRY.
+        inv NTHENTRY.
         assert(k_ key <=? k_ (entry_key ei) = true).
         { assert(-1 < k_ key < Int64.modulus) by (unfold k_; rep_omega).
           destruct ei; simpl in H5; simpl;
@@ -333,14 +343,14 @@ Proof.
               try apply Zaux.Zle_bool_false; unfold k_; omega. }
           apply nth_entry_skipn in NTHENTRY.          
           rewrite skip_S.
-          destruct (skipn_le le i); simpl in NTHENTRY; inv NTHENTRY.
+          destruct (skipn_le le i); autorewrite with sublist in NTHENTRY; inv NTHENTRY.
           simpl. destruct ei; simpl; simpl in H; rewrite H; auto. omega. }
         rewrite unfold_btnode_rep with (n:=n). unfold n.
         Exists ent_end. entailer!.
     + forward.                  (* break *)
-      Exists (numKeys_le le).
+      Exists (Zlength le).
       entailer!.
-      assert(i=numKeys_le le).
+      assert(i=Zlength le).
       { unfold n in H2. simpl in H2.
       apply node_wf_numKeys in H0. simpl in H0.
         rewrite !Int.signed_repr in H4 by rep_omega.
